formulated index_map_rule_39. it is ready to prove now

IndexFunctions.v
@@ -34,6 +34,11 @@ Definition index_map_dom {d r:nat} (s: index_map_spec d r) := d.
 (* Returns upper rang bound for given `index_map_spec` *)
 Definition index_map_range {d r:nat} (s: index_map_spec d r) := r.
 
+Global Instance index_map_equiv {domain range:nat}:
+  Equiv (index_map_spec domain range)
+  :=
+    fun f g => forall (x:nat) (xd: x<domain), f x xd = g x xd.
+
 Fixpoint natrange_list (n:nat) : list nat :=
   match n with
   | 0 => nil
@@ -111,11 +116,10 @@ Admitted.
 Section Primitive_Functions.
   
   Program Definition identity_index_map
-          {domain range: nat}
-          {drdep: domain ≡ range}:
-    index_map_spec domain range
+          (dr: nat):
+    index_map_spec dr dr
     :=
-      fun i i_dim => i.
+      fun i _ => i.
   
   Program Definition constant_index_map
           {range: nat}
@@ -191,37 +195,73 @@ End Function_Operators.
 Notation "g ∘ f" := (index_map_compose g f) : index_f_scope.
 Notation "x ⊗ y" := (index_map_tensor_product x y) (at level 90) : index_f_scope.
 
+Lemma index_function_proj1_bound
+      {domain range: nat}
+      (f_spec: index_map_spec domain range):
+  forall n (nd: n<domain), proj1_sig (f_spec n nd) < range.
+Proof.
+  auto.
+Qed.
+
 Section Function_Rules.
 
   Local Open Scope index_f_scope.
 
-  (*
-Experiments to check typing:
-  Variable df0 df1 rf0 rf1 dg0 dg1 rg0 rg1:nat.
-  Variable f0: index_map_spec df0 rf0.
-  Variable f1: index_map_spec df1 rf1.
-  Variable g0: index_map_spec dg0 rg0.
-  Variable g1: index_map_spec dg1 rg1.
-  Check(g0 ⊗ g1). (* (dg0 * dg1) (rg0 * rg1) *)
-  Check (f0 ⊗ f1). (* (df0 * df1) (rf0 * rf1) *)
-  Check (f0 ⊗ g0). (* (df0 * dg0) (rf0 * rg0) *)
-  Check (f1 ⊗ g1). (* (df1 * dg1) (rf1 * rg1) *)
-*)
-  
-  Program Lemma index_map_rule_39
-        {df0 df1 rf0 rf1 dg0 dg1 rg0 rg1:nat}
-        {c1: (rg0 * rg1) ≡ (df0 * df1)}
-        {c2: (rf1 * rg1) ≡ (df0 * dg0)}
-        {ls:  (dg0 * dg1) ≡ (rf0 * rf1)}
-        {rs: (df1 * dg1) ≡ (df0 * dg0)}
-        (f0: index_map_spec df0 rf0)
-        (f1: index_map_spec df1 rf1)
-        (g0: index_map_spec dg0 rg0)
-        (g1: index_map_spec dg1 rg1):
-    (f0 ⊗ f1) ∘ (g0 ⊗ g1) = (f0 ⊗ g0) ∘ (f1 ⊗ g1).
+  Section rule_39.
+    Variable df0 df1 rf0 rf1 dg0 dg1 rg0 rg1:nat.
+    Variable g0: index_map_spec dg0 rg0.
+    Variable g1: index_map_spec dg1 rg1.
     
-  Local Close Scope index_f_scope.
+    
+    Variable f0: index_map_spec df0 rf0.
+    Variable f1: index_map_spec df1 rf1.
+
+    Variable ndg1: 0 ≢ dg1.
+    Variable ndf1: 0 ≢ df1.
+    Variable ls:  (dg0 * dg1) ≡ (rf0 * rf1).
+    Variable lc1: (rg0 * rg1) ≡ (df0 * df1).
+    
+    Definition f0f1  := index_map_tensor_product f0 f1 (nz:=ndf1).
+    Definition g0g1 := (index_map_tensor_product g0 g1 (nz:=ndg1)).
+
+    Program Definition lhs := f0f1 ∘ g0g1.
+    Next Obligation.
+      assert ((proj1_sig (g0 (fst (divmod x (pred dg1) 0 (pred dg1)))
+                                          (index_map_tensor_product_obligation_1 dg0 dg1 rg0 rg1 ndg1 g0 g1 x x0))) < rg0) by apply index_function_proj1_bound.
+      generalize dependent (proj1_sig (g0 (fst (divmod x (pred dg1) 0 (pred dg1)))
+                                          (index_map_tensor_product_obligation_1 dg0 dg1 rg0 rg1 ndg1 g0 g1 x x0))).
+
+      assert ((proj1_sig (g1 (pred dg1 - snd (divmod x (pred dg1) 0 (pred dg1)))
+                                          (index_map_tensor_product_obligation_2 dg0 dg1 rg0 rg1 ndg1 g0 g1 x x0))) < rg1) by apply index_function_proj1_bound.
+      generalize dependent (proj1_sig (g1 (pred dg1 - snd (divmod x (pred dg1) 0 (pred dg1)))
+                                          (index_map_tensor_product_obligation_2 dg0 dg1 rg0 rg1 ndg1 g0 g1 x x0))).
+      intros.
+      nia.
+    Defined.
+
+
+
+    Variable rc1: rg0 ≡ df0.
+    Program Definition f0cg0 := f0 ∘ g0.
+
+    Variable rc2: rg1 ≡ df1.
+    Program Definition f1cg1 := f1 ∘ g1.
+
+    Variable nf1cg1: 0 ≢ index_map_dom f1cg1.
+    Program Definition rhs :=  index_map_tensor_product
+                                 f0cg0
+                                 f1cg1
+                                 (nz := nf1cg1).
+
+    Program Lemma index_map_rule_39
+      : lhs = rhs.
+    Proof.
+      
+    Qed.
+  End rule_39.
   
+  Local Close Scope index_f_scope.
+        
 End Function_Rules.
   
 
